elaboration for all binds, lifts, frame, and sub, wip on proof of top-level soundness for the new combinators

pulse/examples/dsls/mini_steel/Pulse.Elaborate.fst
@@ -10,19 +10,6 @@ open Pulse.Typing
 
 let return_lid = mk_steel_wrapper_lid "return_stt"
 let return_noeq_lid = mk_steel_wrapper_lid "return_stt_noeq"
-
-let bind_lid = mk_steel_wrapper_lid "bind_stt"
-let bind_fv = R.pack_fv bind_lid
-let bind_univ_inst u1 u2 = R.pack_ln (R.Tv_UInst bind_fv [u1;u2])
-
-let frame_lid = mk_steel_wrapper_lid "frame_stt"
-let frame_fv = R.pack_fv frame_lid
-let frame_univ_inst u = R.pack_ln (R.Tv_UInst (R.pack_fv frame_lid) [u])
-
-let subsumption_lid = mk_steel_wrapper_lid "sub_stt"
-let subsumption_fv = R.pack_fv subsumption_lid
-let subsumption_univ_inst u = R.pack_ln (R.Tv_UInst subsumption_fv [u])
-
 let mk_return (u:R.universe) (ty:R.term) (t:R.term) 
   : R.term
   = let head = R.pack_ln (R.Tv_UInst (R.pack_fv return_lid) [u]) in
@@ -33,13 +20,38 @@ let mk_return_noeq (u:R.universe) (ty:R.term) (t:R.term)
   = let head = R.pack_ln (R.Tv_UInst (R.pack_fv return_noeq_lid) [u]) in
     R.mk_app head [(ty, R.Q_Implicit); (t, R.Q_Explicit)]
 
-let mk_bind (u1 u2:universe)
-            (ty1 ty2:R.term)
-            (pre1 post1: R.term)
-            (post2: R.term)
-            (t1 t2:R.term) 
+// Wrapper.lift_stt_atomic<u> #a #pre #post e
+let mk_lift_atomic_stt (u:R.universe) (a pre post e:R.term)  =
+  let open R in
+  let lid = mk_steel_wrapper_lid "lift_stt_atomic" in
+  let t = pack_ln (R.Tv_UInst (R.pack_fv lid) [u]) in
+  let t = pack_ln (R.Tv_App t (a, Q_Implicit)) in
+  let t = pack_ln (R.Tv_App t (pre, Q_Implicit)) in
+  let t = pack_ln (R.Tv_App t (post, Q_Implicit)) in
+  pack_ln (R.Tv_App t (e, Q_Explicit))
+
+// Wrapper.lift_stt_ghost<u> #a #opened #pre #post e reveal_a
+let mk_lift_ghost_atomic (u:R.universe) (a opened pre post e reveal_a:R.term) =
+  let open R in
+  let lid = mk_steel_wrapper_lid "lift_stt_ghost" in
+  let t = pack_ln (R.Tv_UInst (R.pack_fv lid) [u]) in
+  let t = pack_ln (R.Tv_App t (a, Q_Implicit)) in
+  let t = pack_ln (R.Tv_App t (opened, Q_Implicit)) in
+  let t = pack_ln (R.Tv_App t (pre, Q_Implicit)) in
+  let t = pack_ln (R.Tv_App t (post, Q_Implicit)) in
+  let t = pack_ln (R.Tv_App t (e, Q_Explicit)) in
+  pack_ln (R.Tv_App t (reveal_a, Q_Explicit))
+
+// Wrapper.bind_stt<u1, u2> #a #b #pre1 #post1 #post2 e1 e2
+let mk_bind_stt
+  (u1 u2:R.universe)
+  (ty1 ty2:R.term)
+  (pre1 post1: R.term)
+  (post2: R.term)
+  (t1 t2:R.term) 
   : R.term
-  = let head = bind_univ_inst (elab_universe u1) (elab_universe u2) in
+  = let bind_lid = mk_steel_wrapper_lid "bind_stt" in
+    let head = R.pack_ln (R.Tv_UInst (R.pack_fv bind_lid) [u1;u2]) in
     R.mk_app
       (R.mk_app
         (R.mk_app
@@ -55,14 +67,69 @@ let mk_bind (u1 u2:universe)
         [(t1, R.Q_Explicit)])
       [(t2, R.Q_Explicit)]
 
-let mk_frame (u:universe)
-             (ty:R.term)
-             (pre: R.term)
-             (post: R.term)
-             (frame: R.term)
-             (t:R.term) 
+// Wrapper.bind_sttg<u1, u2> #a #b #opened #pre1 #post1 #post2 e1 e2
+let mk_bind_ghost
+  (u1 u2:R.universe)
+  (a b opened pre1 post1 post2 e1 e2:R.term) =
+  let open R in
+  let bind_lid = mk_steel_wrapper_lid "bind_sttg" in
+  let t = R.pack_ln (R.Tv_UInst (R.pack_fv bind_lid) [u1;u2]) in
+  let t = pack_ln (R.Tv_App t (a, Q_Implicit)) in
+  let t = pack_ln (R.Tv_App t (b, Q_Implicit)) in
+  let t = pack_ln (R.Tv_App t (opened, Q_Implicit)) in
+  let t = pack_ln (R.Tv_App t (pre1, Q_Implicit)) in
+  let t = pack_ln (R.Tv_App t (post1, Q_Implicit)) in
+  let t = pack_ln (R.Tv_App t (post2, Q_Implicit)) in
+  let t = pack_ln (R.Tv_App t (e1, Q_Explicit)) in
+  pack_ln (R.Tv_App t (e2, Q_Explicit))
+
+// Wrapper.bind_stt_ghost_atomic<u1, u2> #a #b #opened #pre1 #post1 #post2 e1 e2 reveal_a
+let mk_bind_ghost_atomic
+  (u1 u2:R.universe)
+  (a b opened pre1 post1 post2 e1 e2 reveal_a:R.term) =
+  let open R in
+  let bind_lid = mk_steel_wrapper_lid "bind_stt_ghost_atomic" in
+  let t = R.pack_ln (R.Tv_UInst (R.pack_fv bind_lid) [u1;u2]) in
+  let t = pack_ln (R.Tv_App t (a, Q_Implicit)) in
+  let t = pack_ln (R.Tv_App t (b, Q_Implicit)) in
+  let t = pack_ln (R.Tv_App t (opened, Q_Implicit)) in
+  let t = pack_ln (R.Tv_App t (pre1, Q_Implicit)) in
+  let t = pack_ln (R.Tv_App t (post1, Q_Implicit)) in
+  let t = pack_ln (R.Tv_App t (post2, Q_Implicit)) in
+  let t = pack_ln (R.Tv_App t (e1, Q_Explicit)) in
+  let t = pack_ln (R.Tv_App t (e2, Q_Explicit)) in
+  pack_ln (R.Tv_App t (reveal_a, Q_Explicit))
+
+// Wrapper.bind_stt_atomic_ghost<u1, u2> #a #b #opened #pre1 #post1 #post2 e1 e2 reveal_b
+let mk_bind_atomic_ghost
+  (u1 u2:R.universe)
+  (a b opened pre1 post1 post2 e1 e2 reveal_b:R.term) =
+  let open R in
+  let bind_lid = mk_steel_wrapper_lid "bind_stt_atomic_ghost" in
+  let t = R.pack_ln (R.Tv_UInst (R.pack_fv bind_lid) [u1;u2]) in
+  let t = pack_ln (R.Tv_App t (a, Q_Implicit)) in
+  let t = pack_ln (R.Tv_App t (b, Q_Implicit)) in
+  let t = pack_ln (R.Tv_App t (opened, Q_Implicit)) in
+  let t = pack_ln (R.Tv_App t (pre1, Q_Implicit)) in
+  let t = pack_ln (R.Tv_App t (post1, Q_Implicit)) in
+  let t = pack_ln (R.Tv_App t (post2, Q_Implicit)) in
+  let t = pack_ln (R.Tv_App t (e1, Q_Explicit)) in
+  let t = pack_ln (R.Tv_App t (e2, Q_Explicit)) in
+  pack_ln (R.Tv_App t (reveal_b, Q_Explicit))
+
+// Wrapper.frame_stt<u> #ty #pre #post frame t
+let mk_frame_stt
+  (u:R.universe)
+  (ty:R.term)
+  (pre: R.term)
+  (post: R.term)
+  (frame: R.term)
+  (t:R.term) 
   : R.term
-  = let head = frame_univ_inst (elab_universe u) in
+  = let frame_lid = mk_steel_wrapper_lid "frame_stt" in
+    let frame_fv = R.pack_fv frame_lid in
+    let frame_univ_inst u = R.pack_ln (R.Tv_UInst (R.pack_fv frame_lid) [u]) in
+    let head = frame_univ_inst u in
     R.mk_app
       (R.mk_app
         (R.mk_app
@@ -73,13 +140,42 @@ let mk_frame (u:universe)
         [(frame, R.Q_Explicit)])
       [(t, R.Q_Explicit)]
 
-let mk_sub (u:R.universe)
-           (ty:R.term)
-           (pre1 pre2: R.term)
-           (post1 post2: R.term)
-           (t:R.term) 
+// Wrapper.frame_stt_atomic<u> #a #opened #pre #post frame e
+let mk_frame_stt_atomic (u:R.universe) (a opened pre post frame e:R.term)  =
+  let open R in
+  let lid = mk_steel_wrapper_lid "frame_stt_atomic" in
+  let t = pack_ln (R.Tv_UInst (R.pack_fv lid) [u]) in
+  let t = pack_ln (R.Tv_App t (a, Q_Implicit)) in
+  let t = pack_ln (R.Tv_App t (opened, Q_Implicit)) in
+  let t = pack_ln (R.Tv_App t (pre, Q_Implicit)) in
+  let t = pack_ln (R.Tv_App t (post, Q_Implicit)) in
+  let t = pack_ln (R.Tv_App t (frame, Q_Explicit)) in
+  pack_ln (R.Tv_App t (e, Q_Explicit))
+
+// Wrapper.frame_stt_ghost<u> #a #opened #pre #post frame e
+let mk_frame_stt_ghost (u:R.universe) (a opened pre post frame e:R.term)  =
+  let open R in
+  let lid = mk_steel_wrapper_lid "frame_stt_ghost" in
+  let t = pack_ln (R.Tv_UInst (R.pack_fv lid) [u]) in
+  let t = pack_ln (R.Tv_App t (a, Q_Implicit)) in
+  let t = pack_ln (R.Tv_App t (opened, Q_Implicit)) in
+  let t = pack_ln (R.Tv_App t (pre, Q_Implicit)) in
+  let t = pack_ln (R.Tv_App t (post, Q_Implicit)) in
+  let t = pack_ln (R.Tv_App t (frame, Q_Explicit)) in
+  pack_ln (R.Tv_App t (e, Q_Explicit))
+
+// Wrapper.sub_stt<u> #ty #pre1 pre2 #post1 post2 () () e
+let mk_sub_stt
+  (u:R.universe)
+  (ty:R.term)
+  (pre1 pre2: R.term)
+  (post1 post2: R.term)
+  (t:R.term) 
   : R.term
-  = let head = subsumption_univ_inst u in
+  = let subsumption_lid = mk_steel_wrapper_lid "sub_stt" in
+    let subsumption_fv = R.pack_fv subsumption_lid in
+    let subsumption_univ_inst u = R.pack_ln (R.Tv_UInst subsumption_fv [u]) in
+    let head = subsumption_univ_inst u in
     R.mk_app
      (R.mk_app 
       (R.mk_app
@@ -96,24 +192,158 @@ let mk_sub (u:R.universe)
       [(`(), R.Q_Explicit)])
      [(t, R.Q_Explicit)]
 
-let elab_bind (c1 c2:pure_comp_st) (e1 e2:R.term) =
-  let c1 = st_comp_of_comp c1 in
-  let c2 = st_comp_of_comp c2 in
-  let ty1 = elab_pure c1.res in
-  let ty2 = elab_pure c2.res in
-  mk_bind c1.u c2.u
-          ty1 ty2
-          (elab_pure c1.pre)
-          (mk_abs ty1 R.Q_Explicit (elab_pure c1.post))
-          (mk_abs ty2 R.Q_Explicit (elab_pure c2.post))
-          e1 e2
+// Wrapper.sub_stt_atomic<u> #a #opened #pre1 pre2 #post1 post2 () () e
+let mk_sub_stt_atomic (u:R.universe) (a opened pre1 pre2 post1 post2 e:R.term)  =
+  let open R in
+  let lid = mk_steel_wrapper_lid "sub_stt_atomic" in
+  let t = pack_ln (R.Tv_UInst (R.pack_fv lid) [u]) in
+  let t = pack_ln (R.Tv_App t (a, Q_Implicit)) in
+  let t = pack_ln (R.Tv_App t (opened, Q_Implicit)) in
+  let t = pack_ln (R.Tv_App t (pre1, Q_Implicit)) in
+  let t = pack_ln (R.Tv_App t (pre2, Q_Explicit)) in
+  let t = pack_ln (R.Tv_App t (post1, Q_Implicit)) in
+  let t = pack_ln (R.Tv_App t (post2, Q_Explicit)) in
+  let t = pack_ln (R.Tv_App t (`(), Q_Explicit)) in
+  let t = pack_ln (R.Tv_App t (`(), Q_Explicit)) in
+  pack_ln (R.Tv_App t (e, Q_Explicit))
 
-let rec elab_src_typing (#f:RT.fstar_top_env)
-                        (#g:env)
-                        (#t:term)
-                        (#c:pure_comp)
-                        (d:src_typing f g t c)
+// Wrapper.sub_stt_ghost<u> #a #opened #pre1 pre2 #post1 post2 () () e
+let mk_sub_stt_ghost (u:R.universe) (a opened pre1 pre2 post1 post2 e:R.term)  =
+  let open R in
+  let lid = mk_steel_wrapper_lid "sub_stt_ghost" in
+  let t = pack_ln (R.Tv_UInst (R.pack_fv lid) [u]) in
+  let t = pack_ln (R.Tv_App t (a, Q_Implicit)) in
+  let t = pack_ln (R.Tv_App t (opened, Q_Implicit)) in
+  let t = pack_ln (R.Tv_App t (pre1, Q_Implicit)) in
+  let t = pack_ln (R.Tv_App t (pre2, Q_Explicit)) in
+  let t = pack_ln (R.Tv_App t (post1, Q_Implicit)) in
+  let t = pack_ln (R.Tv_App t (post2, Q_Explicit)) in
+  let t = pack_ln (R.Tv_App t (`(), Q_Explicit)) in
+  let t = pack_ln (R.Tv_App t (`(), Q_Explicit)) in
+  pack_ln (R.Tv_App t (e, Q_Explicit))
+
+let elab_frame (c:pure_comp_st) (frame:pure_term) (e:R.term) =
+  let u = elab_universe (comp_u c) in
+  let ty = elab_pure (comp_res c) in
+  let pre = elab_pure (comp_pre c) in
+  let post = elab_pure (comp_post c) in
+  if C_ST? c
+  then mk_frame_stt u ty pre (mk_abs ty R.Q_Explicit post) (elab_pure frame) e
+  else let opened = elab_pure (comp_inames c) in      
+       if C_STAtomic? c
+       then mk_frame_stt_atomic u ty opened pre (mk_abs ty R.Q_Explicit post) (elab_pure frame) e
+       else let _ = assert (C_STGhost? c) in
+            mk_frame_stt_ghost u ty opened pre (mk_abs ty R.Q_Explicit post) (elab_pure frame) e
+
+let elab_sub (c1 c2:pure_comp_st) (e:R.term) =
+  let ty = elab_pure (comp_res c1) in
+  let u = elab_universe (comp_u c1) in
+  let pre1 = elab_pure (comp_pre c1) in
+  let pre2 = elab_pure (comp_pre c2) in
+  let post1 = mk_abs ty R.Q_Explicit (elab_pure (comp_post c1)) in
+  let post2 = mk_abs ty R.Q_Explicit (elab_pure (comp_post c2)) in
+  if C_ST? c1
+  then mk_sub_stt u ty pre1 pre2 post1 post2 e
+  else let opened = elab_pure (comp_inames c1) in
+       if C_STAtomic? c1
+       then mk_sub_stt_atomic u ty opened pre1 pre2 post1 post2 e
+       else let _ = assert (C_STGhost? c1) in
+            mk_sub_stt_ghost u ty opened pre1 pre2 post1 post2 e
+
+#push-options "--z3rlimit_factor 4"
+let rec elab_lift #f #g #c1 #c2 (d:lift_comp f g c1 c2) (e:R.term)
+  : Tot R.term (decreases d) =
+
+  match d with
+  | Lift_STAtomic_ST _ _ ->
+    let t = elab_pure (comp_res c1) in
+    mk_lift_atomic_stt
+      (elab_universe (comp_u c1))
+      (elab_pure (comp_res c1))
+      t
+      (mk_abs t R.Q_Explicit (elab_pure (comp_post c1)))
+      e
+      
+  | Lift_STGhost_STAtomic _ _ (| reveal_a, reveal_a_typing |) ->
+    let t = elab_pure (comp_res c1) in
+    mk_lift_ghost_atomic
+      (elab_universe (comp_u c1))
+      t
+      (elab_pure (comp_inames c1))
+      (elab_pure (comp_pre c1))
+      (mk_abs t R.Q_Explicit (elab_pure (comp_post c1)))
+      e
+      (elab_src_typing reveal_a_typing)
+
+and elab_bind #f #g #x #c1 #c2 #c (bc:bind_comp f g x c1 c2 c) (e1 e2:R.term)
+  : Tot R.term (decreases bc) =
+
+  let t1 = elab_pure (comp_res c1) in
+  let t2 = elab_pure (comp_res c2) in
+
+  match bc with
+  | Bind_comp _ _ _ _ _ _ _ ->
+    if C_ST? c1
+    then
+      mk_bind_stt
+        (elab_universe (comp_u c1))
+        (elab_universe (comp_u c2))
+        t1 t2
+        (elab_pure (comp_pre c1))
+        (mk_abs t1 R.Q_Explicit (elab_pure (comp_post c1)))
+        (mk_abs t2 R.Q_Explicit (elab_pure (comp_post c2)))
+        e1 e2
+    else 
+      mk_bind_ghost
+        (elab_universe (comp_u c1))
+        (elab_universe (comp_u c2))
+        t1 t2
+        (elab_pure (comp_inames c1))
+        (elab_pure (comp_pre c1))
+        (mk_abs t1 R.Q_Explicit (elab_pure (comp_post c1)))
+        (mk_abs t2 R.Q_Explicit (elab_pure (comp_post c2)))
+        e1 e2
+
+  | Bind_comp_ghost_l _ _ _ _ (| reveal_a, reveal_a_typing |) _ _ _ ->
+    mk_bind_ghost_atomic
+      (elab_universe (comp_u c1))
+      (elab_universe (comp_u c2))
+      t1 t2
+      (elab_pure (comp_inames c1))
+      (elab_pure (comp_pre c1))
+      (mk_abs t1 R.Q_Explicit (elab_pure (comp_post c1)))
+      (mk_abs t2 R.Q_Explicit (elab_pure (comp_post c2)))
+      e1 e2
+      (elab_src_typing reveal_a_typing)
+
+  | Bind_comp_ghost_r _ _ _ _ (| reveal_b, reveal_b_typing |) _ _ _ ->
+    mk_bind_atomic_ghost
+      (elab_universe (comp_u c1))
+      (elab_universe (comp_u c2))
+      t1 t2
+      (elab_pure (comp_inames c1))
+      (elab_pure (comp_pre c1))
+      (mk_abs t1 R.Q_Explicit (elab_pure (comp_post c1)))
+      (mk_abs t2 R.Q_Explicit (elab_pure (comp_post c2)))
+      e1 e2
+      (elab_src_typing reveal_b_typing)
+
+  | Bind_lift_l _ _ _ _ _ lc _ bc ->
+    let e1 = elab_lift lc e1 in
+    elab_bind bc e1 e2
+
+  | Bind_lift_r _ _ _ _ _ lc _ bc ->
+    let e2 = elab_lift lc e2 in
+    elab_bind bc e1 e2
+
+and elab_src_typing
+  (#f:RT.fstar_top_env)
+  (#g:env)
+  (#t:term)
+  (#c:pure_comp)
+  (d:src_typing f g t c)
   : Tot R.term (decreases d)
+
   = match d with
     | T_Tot _ _ _ _ -> elab_pure t
 
@@ -133,25 +363,15 @@ let rec elab_src_typing (#f:RT.fstar_top_env)
     | T_ReturnNoEq _ _ ty u t_typing _ ->
       mk_return_noeq (elab_universe u) (elab_pure ty) (elab_src_typing t_typing)
 
-    | T_Bind _ e1 e2 c1 c2 x c e1_typing t_typing e2_typing _bc ->
-      if C_ST? c1 && C_ST? c2
-      then
-        let e1 = elab_src_typing e1_typing in
-        let e2 = elab_src_typing e2_typing in
-        let ty1 = elab_pure (comp_res c1) in
-        elab_bind c1 c2 e1 (mk_abs ty1 R.Q_Explicit (RT.close_term e2 x))
-      else admit ()
+    | T_Bind _ e1 e2 c1 c2 x c e1_typing t_typing e2_typing bc ->
+      let e1 = elab_src_typing e1_typing in
+      let e2 = elab_src_typing e2_typing in
+      let ty1 = elab_pure (comp_res c1) in
+      elab_bind bc e1 (mk_abs ty1 R.Q_Explicit (RT.close_term e2 x))
       
     | T_Frame _ _ c frame _frame_typing e_typing ->
-      if C_ST? c
-      then
-        let e = elab_src_typing e_typing in
-        let c = st_comp_of_comp c in
-        let ty = elab_pure c.res in
-        let pre = elab_pure c.pre in
-        let post = elab_pure c.post in
-        mk_frame c.u ty pre (mk_abs ty R.Q_Explicit post) (elab_pure frame) e
-      else admit ()
+      let e = elab_src_typing e_typing in
+      elab_frame c frame e
       
     // | T_If _ b e1 e2 _c hyp _ e1_typing e2_typing ->
     //   let b = elab_pure b in
@@ -163,20 +383,9 @@ let rec elab_src_typing (#f:RT.fstar_top_env)
     //                (Pat_Constant C_False, e2)])
 
     | T_Equiv _ _ c1 c2 e_typing _ ->
-      if C_ST? c1 && C_ST? c2
-      then
-        let e = elab_src_typing e_typing in
-        let c1 = st_comp_of_comp c1 in
-        let c2 = st_comp_of_comp c2 in
-        let ty = elab_pure c1.res in
-        mk_sub (elab_universe c1.u)
-               ty
-               (elab_pure c1.pre)
-               (elab_pure c2.pre)
-               (mk_abs ty R.Q_Explicit (elab_pure c1.post))
-               (mk_abs ty R.Q_Explicit (elab_pure c2.post))
-               e
-      else admit ()
+      let e = elab_src_typing e_typing in
+      elab_sub c1 c2 e
+#pop-options
 
 #push-options "--ifuel 2"
 let rec elab_pure_equiv (#f:RT.fstar_top_env)
