pulse/examples/dsls/mini_steel/Pulse.Soundness.Bind.fsti
@@ -10,6 +10,8 @@ open Pulse.Typing
 open Pulse.Elaborate
 open Pulse.Soundness.Common
 
+
+// Wrapper.bind_stt and Wrapper.bind_sttg
 val elab_bind_typing (f:stt_env)
                      (g:env)
                      (c1 c2 c:ln_comp)
@@ -24,4 +26,54 @@ val elab_bind_typing (f:stt_env)
                      (post2_typing: RT.typing (extend_env_l f g) 
                                               (elab_comp_post c2)
                                               (post2_type_bind (elab_pure (comp_res c2))))
-  : GTot (RT.typing (extend_env_l f g) (elab_bind c1 c2 r1 r2) (elab_pure_comp c))
+  : Ghost (RT.typing (extend_env_l f g) (elab_bind bc r1 r2) (elab_pure_comp c))
+          (requires Bind_comp? bc)
+          (ensures fun _ -> True)
+
+// Wrapper.bind_stt_ghost_atomic
+val elab_bind_ghost_l_typing
+  (f:stt_env)
+  (g:env)
+  (c1 c2 c:ln_comp)
+  (x:var{~ (x `Set.mem` freevars_comp c1)})
+  (r1:R.term)
+  (r1_typing:RT.typing (extend_env_l f g) r1 (elab_pure_comp c1))
+  (r2:R.term)
+  (r2_typing:RT.typing (extend_env_l f g) r2
+                       (elab_pure (Tm_Arrow (null_binder (comp_res c1)) None (close_pure_comp c2 x))))
+  (bc:bind_comp f g x c1 c2 c)
+  (t2_typing:RT.typing (extend_env_l f g) (elab_pure (comp_res c2))
+                       (RT.tm_type (elab_universe (comp_u c2))))
+  (post2_typing:RT.typing (extend_env_l f g) (elab_comp_post c2)
+                          (post2_type_bind (elab_pure (comp_res c2))))
+  (reveal_a:R.term)
+  (reveal_a_typing:RT.typing (extend_env_l f g) reveal_a
+                             (non_informative_witness_rt (elab_universe (comp_u c1))
+                                                         (elab_pure (comp_res c1))))
+  : Ghost (RT.typing (extend_env_l f g) (elab_bind bc r1 r2) (elab_pure_comp c))
+          (requires Bind_comp_ghost_l? bc)
+          (ensures fun _ -> True)
+
+// Wrapper.bind_stt_atomic_ghost
+val elab_bind_ghost_r_typing
+  (f:stt_env)
+  (g:env)
+  (c1 c2 c:ln_comp)
+  (x:var{~ (x `Set.mem` freevars_comp c1)})
+  (r1:R.term)
+  (r1_typing:RT.typing (extend_env_l f g) r1 (elab_pure_comp c1))
+  (r2:R.term)
+  (r2_typing:RT.typing (extend_env_l f g) r2
+                       (elab_pure (Tm_Arrow (null_binder (comp_res c1)) None (close_pure_comp c2 x))))
+  (bc:bind_comp f g x c1 c2 c)
+  (t2_typing:RT.typing (extend_env_l f g) (elab_pure (comp_res c2))
+                       (RT.tm_type (elab_universe (comp_u c2))))
+  (post2_typing:RT.typing (extend_env_l f g) (elab_comp_post c2)
+                          (post2_type_bind (elab_pure (comp_res c2))))
+  (reveal_b:R.term)
+  (reveal_b_typing:RT.typing (extend_env_l f g) reveal_b
+                             (non_informative_witness_rt (elab_universe (comp_u c2))
+                                                         (elab_pure (comp_res c2))))
+  : Ghost (RT.typing (extend_env_l f g) (elab_bind bc r1 r2) (elab_pure_comp c))
+          (requires Bind_comp_ghost_r? bc)
+          (ensures fun _ -> True)
